lib changes

lib/fst/Lib.IntTypes.fst
@@ -19,6 +19,13 @@ let sec_int_t (t:inttype) = pub_int_t t
 
 let sec_int_v #t (u:sec_int_t t) = pub_int_v #t u
 
+let uint_v #t #l (u:uint_t t l) : n:nat{n <= maxint t} =
+  match l with
+  | PUB -> pub_int_v #t u
+  | SEC -> sec_int_v #t u
+
+let uint_v_pub_lemma #t u = ()
+
 let uintv_extensionality #t #l a b =
   match t with
   | U1   -> ()
@@ -156,6 +163,8 @@ let incr #t #l a =
   | U64 -> (UInt64.add a 0x1uL)
   | U128 -> (UInt128.add a (UInt128.uint_to_t 1))
 
+let incr_lemma #t #l a = ()
+
 let mul_mod #t #l a b =
   match t with
   | U1 -> (UInt8.mul_mod a b)
@@ -174,7 +183,11 @@ let mul #t #l a b =
   | U32 -> (UInt32.mul a b)
   | U64 -> (UInt64.mul a b)
 
+let mul_lemma #t #l a b = ()
+
 let mul64_wide a b = UInt128.mul_wide a b
+
+let mul64_wide_lemma a b = ()
 
 let sub_mod #t #l a b =
   match t with
@@ -185,14 +198,18 @@ let sub_mod #t #l a b =
   | U64 -> (UInt64.sub_mod a b)
   | U128 -> (UInt128.sub_mod a b)
 
+let sub_mod_lemma #t #l a b = ()
+
 let sub #t #l a b =
   match t with
-  | U1 -> (UInt8.sub a b)
+  | U1 -> (UInt8.sub a b) 
   | U8 -> (UInt8.sub a b)
   | U16 -> (UInt16.sub a b)
   | U32 -> (UInt32.sub a b)
   | U64 -> (UInt64.sub a b)
   | U128 -> (UInt128.sub a b)
+
+let sub_lemma #t #l a b = ()
 
 let decr #t #l a =
   match t with
@@ -203,9 +220,11 @@ let decr #t #l a =
   | U64 -> (UInt64.sub a 0x1uL)
   | U128 -> (UInt128.sub a (UInt128.uint_to_t 1))
 
+let decr_lemma #t #l a = ()
+
 let logxor #t #l a b =
   match t with
-  | U1 -> (UInt8.logxor a b)
+  | U1 -> (UInt8.logxor a b) 
   | U8 -> (UInt8.logxor a b)
   | U16 -> (UInt16.logxor a b)
   | U32 -> (UInt32.logxor a b)
@@ -350,6 +369,8 @@ let div #t x y =
   | U32 -> UInt32.div x y
   | U64 -> UInt64.div x y
 
+let div_lemma #t x y = ()
+
 let mod #t x y =
   match t with
   | U1  -> UInt8.rem x y
@@ -357,6 +378,8 @@ let mod #t x y =
   | U16 -> UInt16.rem x y
   | U32 -> UInt32.rem x y
   | U64 -> UInt64.rem x y
+
+let mod_lemma #t x y = ()
 
 let eq #t x y =
   match t with
@@ -367,6 +390,8 @@ let eq #t x y =
   | U64 -> UInt64.eq x y
   | U128 -> UInt128.eq x y
 
+let eq_lemma #t x y = ()
+
 let ne #t x y =
   match t with
   | U1  -> not (UInt8.eq x y)
@@ -375,6 +400,8 @@ let ne #t x y =
   | U32 -> not (UInt32.eq x y)
   | U64 -> not (UInt64.eq x y)
   | U128 -> not (UInt128.eq x y)
+
+let ne_lemma #t x y = ()
 
 let lt #t x y =
   match t with
@@ -385,6 +412,8 @@ let lt #t x y =
   | U64 -> UInt64.lt x y
   | U128 -> UInt128.lt x y
 
+let lt_lemma #t x y = ()
+
 let lte #t x y =
   match t with
   | U1  -> UInt8.lte x y
@@ -393,6 +422,8 @@ let lte #t x y =
   | U32 -> UInt32.lte x y
   | U64 -> UInt64.lte x y
   | U128 -> UInt128.lte x y
+
+let lte_lemma #t x y = ()
 
 let gt #t x y =
   match t with
@@ -403,6 +434,8 @@ let gt #t x y =
   | U64 -> UInt64.gt x y
   | U128 -> UInt128.gt x y
 
+let gt_lemma #t x y = ()
+
 let gte #t x y =
   match t with
   | U1  -> UInt8.gte x y
@@ -412,3 +445,4 @@ let gte #t x y =
   | U64 -> UInt64.gte x y
   | U128 -> UInt128.gte x y
 
+let gte_lemma #t x y = ()
